theories/System/PGS.v
@@ -1,9 +1,1 @@
-Require Import PnV.Prelude.Prelude.
-Require Import PnV.Data.FiniteSet.
-Require Import PnV.Data.FiniteMap.
-Require Import PnV.Data.Graph.
-Require Import PnV.Data.Vector.
 
-#[local] Infix "\in" := E.In : type_scope.
-#[local] Infix "=~=" := is_similar_to : type_scope.
-#[local] Infix "∈" := L.In.
